conversion to Isar/ZF

src/ZF/IMP/Com.thy
@@ -8,34 +8,33 @@ Arithmetic expressions, Boolean expressions, Commands
 And their Operational semantics
 *)
 
-Com = Main +
+theory Com = Main:
 
 (** Arithmetic expressions **)
 consts  loc  :: i
         aexp :: i
 
 datatype <= "univ(loc Un (nat->nat) Un ((nat*nat) -> nat) )"
-  "aexp" = N ("n \\<in> nat")
-         | X ("x \\<in> loc")
-         | Op1 ("f \\<in> nat -> nat", "a \\<in> aexp")
-         | Op2 ("f \\<in> (nat*nat) -> nat", "a0 \\<in> aexp", "a1 \\<in> aexp")
+  "aexp" = N ("n \<in> nat")
+         | X ("x \<in> loc")
+         | Op1 ("f \<in> nat -> nat", "a \<in> aexp")
+         | Op2 ("f \<in> (nat*nat) -> nat", "a0 \<in> aexp", "a1 \<in> aexp")
 
 
 (** Evaluation of arithmetic expressions **)
-consts  evala    :: i
-        "-a->"   :: [i,i] => o                  (infixl 50)
+consts  evala    :: "i"
+        "-a->"   :: "[i,i] => o"                  (infixl 50)
 translations
-    "p -a-> n" == "<p,n> \\<in> evala"
+    "p -a-> n" == "<p,n> \<in> evala"
 inductive
   domains "evala" <= "(aexp * (loc -> nat)) * nat"
-  intrs 
-    N   "[| n \\<in> nat;  sigma \\<in> loc->nat |] ==> <N(n),sigma> -a-> n"
-    X   "[| x \\<in> loc;  sigma \\<in> loc->nat |] ==> <X(x),sigma> -a-> sigma`x"
-    Op1 "[| <e,sigma> -a-> n;  f \\<in> nat -> nat |] ==> <Op1(f,e),sigma> -a-> f`n"
-    Op2 "[| <e0,sigma> -a-> n0;  <e1,sigma>  -a-> n1; f \\<in> (nat*nat) -> nat |] 
-           ==> <Op2(f,e0,e1),sigma> -a-> f`<n0,n1>"
-
-  type_intrs "aexp.intrs@[apply_funtype]"
+  intros 
+    N:   "[| n \<in> nat;  sigma \<in> loc->nat |] ==> <N(n),sigma> -a-> n"
+    X:   "[| x \<in> loc;  sigma \<in> loc->nat |] ==> <X(x),sigma> -a-> sigma`x"
+    Op1: "[| <e,sigma> -a-> n; f \<in> nat -> nat |] ==> <Op1(f,e),sigma> -a-> f`n"
+    Op2: "[| <e0,sigma> -a-> n0;  <e1,sigma>  -a-> n1; f \<in> (nat*nat) -> nat |] 
+          ==> <Op2(f,e0,e1),sigma> -a-> f`<n0,n1>"
+  type_intros aexp.intros apply_funtype
 
 
 (** Boolean expressions **)
@@ -44,35 +43,34 @@ consts  bexp :: i
 datatype <= "univ(aexp Un ((nat*nat)->bool) )"
   "bexp" = true
          | false
-         | ROp  ("f \\<in> (nat*nat)->bool", "a0 \\<in> aexp", "a1 \\<in> aexp")
-         | noti ("b \\<in> bexp")
-         | andi ("b0 \\<in> bexp", "b1 \\<in> bexp")      (infixl 60)
-         | ori  ("b0 \\<in> bexp", "b1 \\<in> bexp")      (infixl 60)
+         | ROp  ("f \<in> (nat*nat)->bool", "a0 \<in> aexp", "a1 \<in> aexp")
+         | noti ("b \<in> bexp")
+         | andi ("b0 \<in> bexp", "b1 \<in> bexp")      (infixl 60)
+         | ori  ("b0 \<in> bexp", "b1 \<in> bexp")      (infixl 60)
 
 
 (** Evaluation of boolean expressions **)
-consts evalb    :: i    
-       "-b->"   :: [i,i] => o                   (infixl 50)
+consts evalb    :: "i"
+       "-b->"   :: "[i,i] => o"                   (infixl 50)
 
 translations
-    "p -b-> b" == "<p,b> \\<in> evalb"
+    "p -b-> b" == "<p,b> \<in> evalb"
 
 inductive
   domains "evalb" <= "(bexp * (loc -> nat)) * bool"
-  intrs (*avoid clash with ML constructors true, false*)
-    tru   "[| sigma \\<in> loc -> nat |] ==> <true,sigma> -b-> 1"
-    fls   "[| sigma \\<in> loc -> nat |] ==> <false,sigma> -b-> 0"
-    ROp   "[| <a0,sigma> -a-> n0; <a1,sigma> -a-> n1; f \\<in> (nat*nat)->bool |] 
+  intros (*avoid clash with ML constructors true, false*)
+    tru:   "[| sigma \<in> loc -> nat |] ==> <true,sigma> -b-> 1"
+    fls:   "[| sigma \<in> loc -> nat |] ==> <false,sigma> -b-> 0"
+    ROp:   "[| <a0,sigma> -a-> n0; <a1,sigma> -a-> n1; f \<in> (nat*nat)->bool |] 
            ==> <ROp(f,a0,a1),sigma> -b-> f`<n0,n1> "
-    noti  "[| <b,sigma> -b-> w |] ==> <noti(b),sigma> -b-> not(w)"
-    andi  "[| <b0,sigma> -b-> w0; <b1,sigma> -b-> w1 |] 
+    noti:  "[| <b,sigma> -b-> w |] ==> <noti(b),sigma> -b-> not(w)"
+    andi:  "[| <b0,sigma> -b-> w0; <b1,sigma> -b-> w1 |] 
           ==> <b0 andi b1,sigma> -b-> (w0 and w1)"
-    ori   "[| <b0,sigma> -b-> w0; <b1,sigma> -b-> w1 |] 
+    ori:   "[| <b0,sigma> -b-> w0; <b1,sigma> -b-> w1 |] 
             ==> <b0 ori b1,sigma> -b-> (w0 or w1)"
-
-  type_intrs "bexp.intrs @   
-              [apply_funtype, and_type, or_type, bool_1I, bool_0I, not_type]"
-  type_elims "[make_elim(evala.dom_subset RS subsetD)]"
+  type_intros  bexp.intros 
+               apply_funtype and_type or_type bool_1I bool_0I not_type
+  type_elims   evala.dom_subset [THEN subsetD, elim_format]
 
 
 (** Commands **)
@@ -80,50 +78,83 @@ consts  com :: i
 
 datatype 
   "com" = skip
-        | asgt  ("x \\<in> loc", "a \\<in> aexp")             (infixl 60)
-        | semic ("c0 \\<in> com", "c1 \\<in> com")            ("_; _"  [60, 60] 10)
-        | while ("b \\<in> bexp", "c \\<in> com")             ("while _ do _"  60)
-        | ifc   ("b \\<in> bexp", "c0 \\<in> com", "c1 \\<in> com")  ("ifc _ then _ else _"  60)
+        | asgt ("x \<in> loc", "a \<in> aexp")             (infixl 60)
+        | semic("c0 \<in> com", "c1 \<in> com")            ("_; _"  [60, 60] 10)
+        | while("b \<in> bexp", "c \<in> com")             ("while _ do _"  60)
+        | ifc  ("b \<in> bexp", "c0 \<in> com", "c1 \<in> com") ("ifc _ then _ else _" 60)
 
 (*Constructor ";" has low precedence to avoid syntactic ambiguities
-  with [| m \\<in> nat; x \\<in> loc; ... |] ==> ...  It usually will need parentheses.*)
+  with [| m \<in> nat; x \<in> loc; ... |] ==> ...  It usually will need parentheses.*)
 
 (** Execution of commands **)
-consts  evalc    :: i
-        "-c->"   :: [i,i] => o                   (infixl 50)
+consts  evalc    :: "i"
+        "-c->"   :: "[i,i] => o"                   (infixl 50)
 
 translations
-       "p -c-> s" == "<p,s> \\<in> evalc"
-
+       "p -c-> s" == "<p,s> \<in> evalc"
 
 inductive
   domains "evalc" <= "(com * (loc -> nat)) * (loc -> nat)"
-  intrs
-    skip    "[| sigma \\<in> loc -> nat |] ==> <skip,sigma> -c-> sigma"
+  intros
+    skip:    "[| sigma \<in> loc -> nat |] ==> <skip,sigma> -c-> sigma"
 
-    assign  "[| m \\<in> nat; x \\<in> loc; <a,sigma> -a-> m |] ==> 
-            <x asgt a,sigma> -c-> sigma(x:=m)"
+    assign:  "[| m \<in> nat; x \<in> loc; <a,sigma> -a-> m |] 
+              ==> <x asgt a,sigma> -c-> sigma(x:=m)"
 
-    semi    "[| <c0,sigma> -c-> sigma2; <c1,sigma2> -c-> sigma1 |] ==> 
-            <c0 ; c1, sigma> -c-> sigma1"
+    semi:    "[| <c0,sigma> -c-> sigma2; <c1,sigma2> -c-> sigma1 |] 
+              ==> <c0 ; c1, sigma> -c-> sigma1"
 
-    ifc1     "[| b \\<in> bexp; c1 \\<in> com; sigma \\<in> loc->nat;   
-                 <b,sigma> -b-> 1; <c0,sigma> -c-> sigma1 |] ==> 
-             <ifc b then c0 else c1, sigma> -c-> sigma1"
+    ifc1:    "[| b \<in> bexp; c1 \<in> com; sigma \<in> loc->nat;   
+                 <b,sigma> -b-> 1; <c0,sigma> -c-> sigma1 |] 
+              ==> <ifc b then c0 else c1, sigma> -c-> sigma1"
 
-    ifc0     "[| b \\<in> bexp; c0 \\<in> com; sigma \\<in> loc->nat;   
-                 <b,sigma> -b-> 0; <c1,sigma> -c-> sigma1 |] ==> 
-             <ifc b then c0 else c1, sigma> -c-> sigma1"
+    ifc0:    "[| b \<in> bexp; c0 \<in> com; sigma \<in> loc->nat;   
+                 <b,sigma> -b-> 0; <c1,sigma> -c-> sigma1 |] 
+               ==> <ifc b then c0 else c1, sigma> -c-> sigma1"
 
-    while0   "[| c \\<in> com; <b, sigma> -b-> 0 |] ==> 
-             <while b do c,sigma> -c-> sigma "
+    while0:   "[| c \<in> com; <b, sigma> -b-> 0 |] 
+               ==> <while b do c,sigma> -c-> sigma"
 
-    while1   "[| c \\<in> com; <b,sigma> -b-> 1; <c,sigma> -c-> sigma2; 
-                <while b do c, sigma2> -c-> sigma1 |] ==> 
-             <while b do c, sigma> -c-> sigma1 "
+    while1:   "[| c \<in> com; <b,sigma> -b-> 1; <c,sigma> -c-> sigma2; 
+                  <while b do c, sigma2> -c-> sigma1 |] 
+               ==> <while b do c, sigma> -c-> sigma1"
 
-  type_intrs "com.intrs @ [update_type]"
-  type_elims "[make_elim(evala.dom_subset RS subsetD),   
-               make_elim(evalb.dom_subset RS subsetD) ]"
+  type_intros  com.intros update_type
+  type_elims   evala.dom_subset [THEN subsetD, elim_format]
+               evalb.dom_subset [THEN subsetD, elim_format]
+
+
+(*** type_intros for evala ***)
+
+lemmas evala_1 [simp] = 
+       evala.dom_subset [THEN subsetD, THEN SigmaD1, THEN SigmaD1]
+lemmas evala_2 [simp] = 
+       evala.dom_subset [THEN subsetD, THEN SigmaD1, THEN SigmaD2]
+lemmas evala_3 [simp] = 
+       evala.dom_subset [THEN subsetD, THEN SigmaD2]
+
+
+(*** type_intros for evalb ***)
+
+lemmas evalb_1 [simp] = 
+       evalb.dom_subset [THEN subsetD, THEN SigmaD1, THEN SigmaD1]
+lemmas evalb_2 [simp] = 
+       evalb.dom_subset [THEN subsetD, THEN SigmaD1, THEN SigmaD2]
+lemmas evalb_3 [simp] = 
+       evalb.dom_subset [THEN subsetD, THEN SigmaD2]
+
+(*** type_intros for evalc ***)
+
+lemmas evalc_1 [simp] = 
+       evalc.dom_subset [THEN subsetD, THEN SigmaD1, THEN SigmaD1]
+lemmas evalc_2 [simp] = 
+       evalc.dom_subset [THEN subsetD, THEN SigmaD1, THEN SigmaD2]
+lemmas evalc_3 [simp] = 
+       evalc.dom_subset [THEN subsetD, THEN SigmaD2]
+
+inductive_cases evala_N_E [elim!]: "<N(n),sigma> -a-> i"
+inductive_cases evala_X_E [elim!]: "<X(x),sigma> -a-> i"
+inductive_cases evala_Op1_E [elim!]: "<Op1(f,e),sigma> -a-> i"
+inductive_cases evala_Op2_E [elim!]: "<Op2(f,a1,a2),sigma>  -a-> i"
 
 end
