src/ZF/Coind/BCR.thy
@@ -1,5 +1,0 @@
-(*  Title:      ZF/Coind/BCR.thy
-    ID:         $Id$
-    Author:     Jacob Frost, Cambridge University Computer Laboratory
-    Copyright   1995  University of Cambridge
-*)
