src/ZF/IMP/Denotation.thy
@@ -6,41 +6,82 @@
 Denotational semantics of expressions & commands
 *)
 
-Denotation = Com + 
+theory Denotation = Com:
+
 
 consts
-  A     :: i => i => i
-  B     :: i => i => i
-  C     :: i => i
-  Gamma :: [i,i,i] => i
+  A     :: "i => i => i"
+  B     :: "i => i => i"
+  C     :: "i => i"
 
-rules   (*NOT definitional*)
-  A_nat_def     "A(N(n)) == (%sigma. n)"
-  A_loc_def     "A(X(x)) == (%sigma. sigma`x)" 
-  A_op1_def     "A(Op1(f,a)) == (%sigma. f`A(a,sigma))"
-  A_op2_def     "A(Op2(f,a0,a1)) == (%sigma. f`<A(a0,sigma),A(a1,sigma)>)"
+constdefs
+  Gamma :: "[i,i,i] => i"
+    "Gamma(b,cden) == (%phi.{io \<in> (phi O cden). B(b,fst(io))=1} Un 
+                         {io \<in> id(loc->nat). B(b,fst(io))=0})"
+
+primrec
+    "A(N(n), sigma) = n"
+    "A(X(x), sigma) = sigma`x" 
+    "A(Op1(f,a), sigma) = f`A(a,sigma)"
+    "A(Op2(f,a0,a1), sigma) = f`<A(a0,sigma),A(a1,sigma)>"
 
 
-  B_true_def    "B(true) == (%sigma. 1)"
-  B_false_def   "B(false) == (%sigma. 0)"
-  B_op_def      "B(ROp(f,a0,a1)) == (%sigma. f`<A(a0,sigma),A(a1,sigma)>)" 
+primrec
+    "B(true, sigma) = 1"
+    "B(false, sigma) = 0"
+    "B(ROp(f,a0,a1), sigma) = f`<A(a0,sigma),A(a1,sigma)>" 
+    "B(noti(b), sigma) = not(B(b,sigma))"
+    "B(b0 andi b1, sigma) = B(b0,sigma) and B(b1,sigma)"
+    "B(b0 ori b1, sigma) = B(b0,sigma) or B(b1,sigma)"
 
 
-  B_not_def     "B(noti(b)) == (%sigma. not(B(b,sigma)))"
-  B_and_def     "B(b0 andi b1) == (%sigma. B(b0,sigma) and B(b1,sigma))"
-  B_or_def      "B(b0 ori b1) == (%sigma. B(b0,sigma) or B(b1,sigma))"
+primrec
+    "C(skip) = id(loc->nat)"
 
-  C_skip_def    "C(skip) == id(loc->nat)"
-  C_assign_def  "C(x asgt a) == {io:(loc->nat)*(loc->nat). 
-                               snd(io) = fst(io)(x := A(a,fst(io)))}"
+    "C(x asgt a) = {io:(loc->nat)*(loc->nat). 
+                    snd(io) = fst(io)(x := A(a,fst(io)))}"
 
-  C_comp_def    "C(c0 ; c1) == C(c1) O C(c0)"
-  C_if_def      "C(ifc b then c0 else c1) == {io \\<in> C(c0). B(b,fst(io))=1} Un 
-                                             {io \\<in> C(c1). B(b,fst(io))=0}"
+    "C(c0 ; c1) = C(c1) O C(c0)"
 
-  Gamma_def     "Gamma(b,c) == (%phi.{io \\<in> (phi O C(c)). B(b,fst(io))=1} Un 
-                                     {io \\<in> id(loc->nat). B(b,fst(io))=0})"
+    "C(ifc b then c0 else c1) = {io \<in> C(c0). B(b,fst(io))=1} Un 
+                                             {io \<in> C(c1). B(b,fst(io))=0}"
 
-  C_while_def   "C(while b do c) == lfp((loc->nat)*(loc->nat), Gamma(b,c))"
+    "C(while b do c) = lfp((loc->nat)*(loc->nat), Gamma(b,C(c)))"
+
+
+(** Type_intr for A **)
+
+lemma A_type [TC]: "[|a \<in> aexp; sigma \<in> loc->nat|] ==> A(a,sigma) \<in> nat"
+by (erule aexp.induct, simp_all)
+
+
+(** Type_intr for B **)
+
+lemma B_type [TC]: "[|b \<in> bexp; sigma \<in> loc->nat|] ==> B(b,sigma) \<in> bool"
+by (erule bexp.induct, simp_all)
+
+(** C_subset **)
+
+lemma C_subset: "c \<in> com ==> C(c) \<subseteq> (loc->nat)*(loc->nat)"
+apply (erule com.induct)
+apply simp_all
+apply (blast dest: lfp_subset [THEN subsetD])+
+done
+
+(** Type_elims for C **)
+
+lemma C_type_D [dest]:
+     "[| <x,y> \<in> C(c); c \<in> com |] ==> x \<in> loc->nat & y \<in> loc->nat"
+by (blast dest: C_subset [THEN subsetD])
+
+lemma C_type_fst [dest]: "[| x \<in> C(c); c \<in> com |] ==> fst(x) \<in> loc->nat"
+by (auto dest!: C_subset [THEN subsetD])
+
+(** bnd_mono (nat->nat*nat->nat,Gamma(b,c) **)
+
+lemma Gamma_bnd_mono: 
+     "cden <= (loc->nat)*(loc->nat) 
+      ==> bnd_mono ((loc->nat)*(loc->nat),Gamma(b,cden))"
+by (unfold bnd_mono_def Gamma_def, blast)
 
 end
