src/ZF/IMP/Equiv.thy
@@ -4,4 +4,84 @@
     Copyright   1994 TUM
 *)
 
-Equiv = Denotation + Com
+theory Equiv = Denotation + Com:
+
+lemma aexp_iff [rule_format]:
+     "[| a \<in> aexp; sigma: loc -> nat |] 
+      ==> ALL n. <a,sigma> -a-> n <-> A(a,sigma) = n"
+apply (erule aexp.induct) 
+apply (force intro!: evala.intros)+
+done
+
+declare aexp_iff [THEN iffD1, simp]
+        aexp_iff [THEN iffD2, intro!]
+
+inductive_cases [elim!]: "<true,sigma> -b-> x"
+inductive_cases [elim!]: "<false,sigma> -b-> x"
+inductive_cases [elim!]: "<ROp(f,a0,a1),sigma> -b-> x"
+inductive_cases [elim!]: "<noti(b),sigma> -b-> x"
+inductive_cases [elim!]: "<b0 andi b1,sigma> -b-> x"
+inductive_cases [elim!]: "<b0 ori b1,sigma> -b-> x"
+
+
+lemma bexp_iff [rule_format]:
+     "[| b \<in> bexp; sigma: loc -> nat |] 
+      ==> ALL w. <b,sigma> -b-> w <-> B(b,sigma) = w"
+apply (erule bexp.induct) 
+apply (auto intro!: evalb.intros)
+done
+
+declare bexp_iff [THEN iffD1, simp]
+        bexp_iff [THEN iffD2, intro!]
+
+lemma com1: "<c,sigma> -c-> sigma' ==> <sigma,sigma'> \<in> C(c)"
+apply (erule evalc.induct)
+apply simp_all
+(* skip *)
+apply fast
+(* assign *)
+apply (simp add: update_type)
+(* comp *)
+apply fast
+(* while *)
+apply (erule Gamma_bnd_mono [THEN lfp_unfold, THEN ssubst, OF C_subset])
+apply (simp add: Gamma_def)
+apply (force ) 
+(* recursive case of while *)
+apply (erule Gamma_bnd_mono [THEN lfp_unfold, THEN ssubst, OF C_subset])
+apply (simp add: Gamma_def)
+apply auto
+done
+
+
+declare B_type [intro!] A_type [intro!]
+declare evalc.intros [intro]
+
+
+lemma com2 [rule_format]: "c \<in> com ==> \<forall>x \<in> C(c). <c,fst(x)> -c-> snd(x)"
+apply (erule com.induct)
+(* skip *)
+apply force
+(* assign *)
+apply force
+(* comp *)
+apply force
+(* while *)
+apply safe
+apply simp_all
+apply (frule Gamma_bnd_mono [OF C_subset], erule Fixedpt.induct, assumption)
+apply (unfold Gamma_def)
+apply force
+(* if *)
+apply auto
+done
+
+
+(**** Proof of Equivalence ****)
+
+lemma com_equivalence:
+     "\<forall>c \<in> com. C(c) = {io:(loc->nat)*(loc->nat). <c,fst(io)> -c-> snd(io)}"
+by (force intro: C_subset [THEN subsetD] elim: com2 dest: com1)
+
+end
+
